Pointer Update

9-Arrays/MinimalBeispiel/minpointerGEP.ll
@@ -1,0 +1,29 @@
+; #MiniSafe
+; globaler Pointer + malloc + read/write mit gep != 0
+target triple = "aarch64-unknown-linux-gnu"
+
+@a = dso_local global ptr null, align 8
+
+; extern malloc
+declare noalias ptr @malloc(i64 noundef)
+
+define dso_local i32 @main() {
+entry:
+  ; 1) Heap anfordern: 8 Bytes (2 * i32)
+  %p = call noalias ptr @malloc(i64 8)
+
+  ; 2) globalen Pointer setzen: a = %p
+  store ptr %p, ptr @a, align 8
+
+  ; 3) Adresse von a[1] (zweites i32) berechnen
+  %p1 = getelementptr inbounds i32, ptr %p, i64 1
+
+  ; 4) a[1] = 7
+  store i32 7, ptr %p1, align 4
+
+  ; 5) v = a[1]
+  %v = load i32, ptr %p1, align 4
+
+  ; 6) Rückgabe: 7
+  ret i32 %v
+}
